theories/νType/νType_index_free.v
@@ -1,0 +1,226 @@
+Require Import List.
+Import Logic.EqNotations ListNotations.
+Require Import Logic.FunctionalExtensionality.
+
+Set Warnings "-notation-overridden".
+From Bonak Require Import SigT Notation RewLemmas HSet LeInductive.
+
+Set Primitive Projections.
+Set Printing Projections.
+Set Keyed Unification.
+Remove Printing Let sigT.
+Remove Printing Let prod.
+
+Section νType.
+Variable arity: HSet.
+
+Section RestrFramesDef.
+
+Inductive PrevLevel :=
+| EmptyPrev : PrevLevel
+| AddPrev (Frame: HSet) (Painting: Frame -> HSet) (rest: PrevLevel) : PrevLevel.
+
+Class RestrFrameTypeBlock := {
+  RestrFrameTypesDef: Type;
+  FrameDef: RestrFrameTypesDef -> HSet;
+}.
+
+(**
+Build the list of pairs of the type RestrFrameTypesDef(n+1,p) of
+restrFrame(n+1,p) for p <= n and of the definition of frame(n+1,p),
+for p <= n+1, in function of effective RestrFrames of these types.
+
+That is, we build for p <= n.+1:
+  p = 0 : { restrFrameTypes = unit ; frame(n+1,0)(restrFrames_{0..0-1}) }
+  p = 1 : { restrFrameTypes = {_:unit & restrFrameType0 ;
+    frame(n+1,1)(restrFrames_{0..0}) }
+  ...
+  p     : { restrFrameTypes = {RestrFrameType0 ... restrFrameType_{p-1}} ;
+    frame_p(restrFrames_{0..p-1}) }
+  n+1   : { restrFrameTypes = {RestrFrameType0 ... restrFrameType_n} ;
+    frame(n+1,n+1)(restrFrames_{0..n})
+*)
+Fixpoint mkRestrFrameTypesAndFrames' (Prev : PrevLevel) : RestrFrameTypeBlock :=
+  match Prev with
+  | EmptyPrev =>
+    {|
+      RestrFrameTypesDef := unit;
+      FrameDef _ := hunit
+    |}
+  | AddPrev FramePrev PaintingPrev rest =>
+    {|
+      RestrFrameTypesDef :=
+        { R: (mkRestrFrameTypesAndFrames' rest).(RestrFrameTypesDef) &T
+          forall q (ε: arity),
+          (mkRestrFrameTypesAndFrames' rest).(FrameDef) R -> FramePrev };
+      FrameDef R :=
+        { d: (mkRestrFrameTypesAndFrames' rest).(FrameDef) R.1 &
+          hforall ε, PaintingPrev (R.2 0 ε d) }
+    |}
+  end.
+
+Definition mkRestrFrameTypes' Prev :=
+  (mkRestrFrameTypesAndFrames' Prev).(RestrFrameTypesDef).
+
+Definition mkFrameOfRestrFrames' Prev: mkRestrFrameTypes' Prev -> HSet :=
+  (mkRestrFrameTypesAndFrames' Prev).(FrameDef).
+
+Inductive PrevExtension (Prev: PrevLevel):  Type :=
+| TopPrev : PrevExtension Prev
+| AddExtraPrev (Frame: HSet) (Painting: Frame -> HSet):
+   PrevExtension (AddPrev Frame Painting Prev) ->
+   PrevExtension Prev.
+
+Inductive RestrFramesExtension Prev (restrs : mkRestrFrameTypes' Prev): PrevExtension Prev -> Type :=
+| Top :
+  forall E: mkFrameOfRestrFrames' Prev restrs -> HSet,
+  RestrFramesExtension Prev restrs (TopPrev Prev)
+| AddRestrFrame FramePrev PaintingPrev extraPrev :
+  forall restr: forall q (ε: arity),
+          mkFrameOfRestrFrames' Prev restrs -> FramePrev.(Dom),
+  RestrFramesExtension (AddPrev FramePrev PaintingPrev Prev) (restrs; restr) extraPrev ->
+  RestrFramesExtension Prev restrs (AddExtraPrev Prev FramePrev PaintingPrev extraPrev).
+
+Fixpoint mkPainting' Prev (restrs': mkRestrFrameTypes' Prev)
+  extraPrev (extrarestrs' : RestrFramesExtension Prev restrs' extraPrev) :
+  mkFrameOfRestrFrames' Prev restrs' -> HSet :=
+  match extrarestrs' in RestrFramesExtension _ _ extraPrev
+     return mkFrameOfRestrFrames' Prev restrs' -> HSet
+  with
+  | Top _ _ E => E
+  | AddRestrFrame _ _ FramePrev PaintingPrev extraPrev restr' extrarestrs' => fun d =>
+       {l: hforall ε, PaintingPrev (restr' 0 ε d) &
+        mkPainting' (AddPrev FramePrev PaintingPrev Prev) (restrs'; restr') extraPrev extrarestrs' (d; l)}
+  end.
+
+Fixpoint mkLevel (Prev : PrevLevel):
+  forall (restrs : mkRestrFrameTypes' Prev)
+    extraPrev (extraRestrs : RestrFramesExtension Prev restrs extraPrev),
+    PrevLevel :=
+  match Prev return forall (restrs : mkRestrFrameTypes' Prev)
+    extraPrev (extraRestrs : RestrFramesExtension Prev restrs extraPrev),
+    PrevLevel
+  with
+  | EmptyPrev => fun _ _ _ => AddPrev hunit (fun _ => hunit) EmptyPrev
+  | AddPrev FramePrev PaintingPrev Prev => fun restrs extraPrev extraRestrs =>
+    AddPrev (mkFrameOfRestrFrames' Prev restrs.1)
+        (mkPainting' Prev restrs.1
+           (AddExtraPrev _ FramePrev PaintingPrev extraPrev)
+            (AddRestrFrame _ _ FramePrev PaintingPrev extraPrev restrs.2 extraRestrs))
+        (mkLevel Prev restrs.1
+            (AddExtraPrev _ FramePrev PaintingPrev extraPrev)
+            (AddRestrFrame _ _ FramePrev PaintingPrev extraPrev restrs.2 extraRestrs))
+  end.
+
+Definition mkRestrFrameTypes Prev restrs extraPrev extraRestrs :=
+  (mkRestrFrameTypesAndFrames' (mkLevel Prev restrs extraPrev extraRestrs)).(RestrFrameTypesDef).
+
+Definition mkFrameOfRestrFrames Prev restrs extraPrev extraRestrs
+  : mkRestrFrameTypes Prev restrs extraPrev extraRestrs -> HSet :=
+  (mkRestrFrameTypesAndFrames' (mkLevel Prev restrs extraPrev extraRestrs)).(FrameDef).
+
+Class CohFrameTypeBlock Prev restrs extraPrev extraRestrs := {
+  CohFrameTypesDef: Type;
+  RestrFramesDef: CohFrameTypesDef -> mkRestrFrameTypes Prev restrs extraPrev extraRestrs
+}.
+
+Variable RestrPainting':
+  forall Prev restrs' FramePrev PaintingPrev
+    (restr': nat -> arity -> mkFrameOfRestrFrames' Prev restrs' -> FramePrev)
+    extraPrev extraRestrs' q
+    ε (d: mkFrameOfRestrFrames' Prev restrs'),
+  mkPainting' Prev restrs' extraPrev extraRestrs' d ->
+  PaintingPrev (restr' q ε d).
+
+Fixpoint mkCohFrameTypesAndRestrFrames Prev :=
+  match Prev return forall (restrFrames' : mkRestrFrameTypes' Prev)
+    extraPrev (extraRestrs : RestrFramesExtension Prev restrFrames' extraPrev),
+    CohFrameTypeBlock Prev restrFrames' extraPrev extraRestrs
+  with
+  | EmptyLevel => fun _ _ _ =>
+    {|
+      CohFrameTypesDef := unit;
+      RestrFramesDef _ := (tt; fun _ _ _ _ _ => tt)
+    |}
+  | AddPrev _ _ _  => fun restrFrames' _ _ =>
+    {|
+      CohFrameTypesDef := { Q:
+        (mkCohFrameTypesAndRestrFrames restrFrames'.1).(CohFrameTypesDef) &T
+        (* statement of cohFrameType(n+2,p) *)
+        forall r q (ε ω: arity) d,
+        restrFrames'.2 q ε
+          (((mkCohFrameTypesAndRestrFrames restrFrames'.1).(RestrFramesDef) Q).2 r  ω d) =
+        restrFrames'.2 r ω
+            (((mkCohFrameTypesAndRestrFrames p _).(RestrFramesDef) Q).2 q.+1 Hq ε d) };
+      RestrFramesDef Q :=
+      (* RestrFrame(n+2,p+1) *)
+      let restrFrame q := match q with
+      | O => fun _ _ _ =>
+        False_rect _ (leI_O_contra Hpq)
+      | S q => fun ε
+        (d: FrameOfRestrFrames p.+1 _) =>
+        (((mkCohFrameTypesAndRestrFrames p _).(RestrFramesDef) Q.1).2
+          q.+1 _ _ ε d.1 as rf in _;
+        fun ω => rew [Painting'' p] Q.2 p q
+          ε ω d.1 in RestrPainting' p q ε _ (d.2 ω)
+          in forall ω, Painting'' p (RestrFrameFromFull'  _ _ _ rf))
+      end in ((mkCohFrameTypesAndRestrFrames p _).(RestrFramesDef) Q.1;
+        restrFrame)
+    |}
+  end.
+
+Class νTypeAux n := {
+  Prev : PrevLevel;
+  restrFrames': mkRestrFrameTypes'  Prev;
+  Level := mkLevel Pref restrFrames' TopPrev Top;
+  restrFrame' p {Hp: p.+1 <~ n.+1} q {Hpq Hq} ε (d: frame' p): frame'' p :=
+    RestrFrameFromFull'  n frame'' painting'' restrFrames' p
+    (Hp := Hp) q (Hpq := Hpq) (Hq := Hq) ε d;
+  restrPainting' {E'} p {Hp: p.+1 <~ n.+1} q {Hpq: p <~ q} {Hq: q <~ n} ε
+    {d: frame' p}:
+    painting' (Hp := leI_down Hp) p d ->
+    painting'' p (restrFrame' p q ε (Hpq := Hpq) (Hq := Hq) d);
+  cohFrames {E'}:
+    mkFullCohFrameTypes n frame'' painting'' restrFrames' E' restrPainting';
+  restrFrames {E'}: mkFullRestrFrameTypes n.+1 frame' painting' :=
+    mkFullRestrFrames n frame'' painting'' restrFrames' E' restrPainting'
+    cohFrames;
+  frame {E'} p {Hp: p <~ n.+2}: HSet :=
+    Frame n frame'' painting'' restrFrames' E' restrPainting'
+    cohFrames p (Hp := Hp);
+  restrFrame {E'} p {Hp: p.+1 <~ n.+2} q {Hpq: p <~ q} {Hq: q <~ n.+1}
+    ε (d: frame p): frame' p :=
+    RestrFrameFromFull n frame'' painting'' restrFrames' E' restrPainting'
+    cohFrames p q ε d (Hp := Hp) (Hpq := Hpq) (Hq := Hq);
+  cohFrameType {E'} {p} {Hp: p.+2 <~ n.+2} {r q} {Hpq: p.+1 <~ q.+1}
+    {Hpr: p.+1 <~ r.+1} {Hrq: r.+1 <~ q.+1} {Hr: r.+1 <~ n.+1}
+    {Hq: q.+1 <~ n.+1} {ε ω d} :=
+    restrFrame' p q ε (restrFrame p r ω d
+      (Hp := leI_down Hp) (Hpq := leI_lower_both Hpr) (Hq := leI_down Hr)) =
+    restrFrame' p r ω (restrFrame p q.+1 ε d);
+  cohFrame {E'} {p} {Hp: p.+2 <~ n.+2} r q {Hpq: p.+1 <~ q.+1}
+    {Hpr Hrq Hr Hq} {ε ω} d:
+    cohFrameType (Hpq := Hpq) (Hrq := Hrq) :=
+    CohFrame n frame'' painting'' restrFrames' E' restrPainting'
+    cohFrames (Hp := Hp) (Hpr := Hpr) (Hrq := Hrq)
+    (Hr := Hr) (Hq := Hq) (ε := ε) (ω := ω) r q d;
+  painting {E'} p {Hp: p <~ n.+2} {E} (d: frame p): HSet :=
+    Painting n frame'' painting'' restrFrames' E'
+    restrPainting' cohFrames p d (Hp := Hp) (E := E);
+  restrPainting {E'} p {Hp: p.+1 <~ n.+2} q {Hpq: p <~ q} {Hq: q <~ n.+1}
+    ε {E} {d: frame p}:
+    painting p d -> painting' p (restrFrame p q ε d) :=
+    RestrPainting n frame'' painting'' restrFrames' E' restrPainting'
+    cohFrames p q ε (Hp := Hp) (Hpq := Hpq) (Hq := Hq) (E := E) d;
+  cohPainting {E'} {p} {Hp: p.+1 <~ n.+1} r q {Hpq: p.+1 <~ q.+1}
+    {Hpr: p.+2 <~ r.+2}
+    {Hrq: r <~ q} {Hr: r.+2 <~ n.+2} {Hq: q.+1 <~ n.+1} {ε ω E}
+    {d: frame p} (c: painting p d (E := E) (E' := E')
+      (Hp := leI_down (leI_down (leI_trans Hpr Hr)))):
+    rew [painting'' p] cohFrame r q d (Hpr := leI_lower_both Hpr)
+      (Hrq := leI_raise_both Hrq) in
+    restrPainting' p q ε (restrPainting p r ω c
+      (Hq := leI_down (leI_lower_both Hr))) =
+    restrPainting' p r ω (restrPainting p q.+1 ε c
+      (Hpq := leI_down Hpq) (Hq := Hq));
+}.
